lib/listTot.fst
@@ -18,7 +18,9 @@ module FStar.List.Tot
 (** Base operations **)
 
 val isEmpty: list 'a -> Tot bool
-let isEmpty l = match l with | [] -> true | _ -> false
+let isEmpty l = match l with
+  | [] -> true
+  | _ -> false
 
 val hd: l:list 'a{is_Cons l} -> Tot 'a
 let hd = function
@@ -38,10 +40,10 @@ let rec nth l n = match l with
   | []     -> None
   | hd::tl -> if n = 0 then Some hd else nth tl (n - 1)
 
-val count: 'a -> list 'a -> Tot nat
-let rec count x = function
+val count: #a:Type0 -> a -> list a -> Tot nat //built-in equality only available at Type0
+let rec count #a x = function
   | [] -> 0
-  | hd::tl -> if x=hd then 1 + (count x tl) else count x tl
+  | hd::tl -> if x=hd then 1 + count x tl else count x tl
 
 val rev_acc: list 'a -> list 'a -> Tot (list 'a)
 let rec rev_acc l acc = match l with
@@ -99,8 +101,8 @@ let rec fold_right f l x = match l with
 
 (** List searching **)
 
-val mem: 'a -> list 'a -> Tot bool //x:'a -> l:list 'a -> b:bool{b==true <==> In x l}
-let rec mem x = function
+val mem: #a:Type0 -> a -> list a -> Tot bool
+let rec mem #a x = function
   | [] -> false
   | hd::tl -> if hd = x then true else mem x tl
 let contains = mem
@@ -109,7 +111,7 @@ val existsb: #a:Type
        -> f:(a -> Tot bool)
        -> list a
        -> Tot bool
-let rec existsb (a:Type) f l = match l with
+let rec existsb #a f l = match l with
  | [] -> false
  | hd::tl -> if f hd then true else existsb f tl
 
@@ -117,7 +119,7 @@ val find: #a:Type
         -> f:(a -> Tot bool)
         -> list a
         -> Tot (option (x:a{f x}))
-let rec find (a:Type) f l = match l with
+let rec find #a f l = match l with
   | [] -> None #(x:a{f x}) //These type annotations are only present because it makes bootstrapping go much faster
   | hd::tl -> if f hd then Some #(x:a{f x}) hd else find f tl
 
@@ -168,27 +170,25 @@ let rec partition f = function
 
 (** [subset la lb] is true if and only if all the elements from [la]
     are also in [lb]. *)
-val subset: #a:Type -> list a -> list a -> Tot bool
-let rec subset la lb =
+val subset: #a:Type0 -> list a -> list a -> Tot bool
+let rec subset #a la lb =
   match la with
   | [] -> true
   | h :: tl ->  mem h lb && subset tl lb
 
-val noRepeats : #a:Type -> list a -> Tot bool
-let rec noRepeats la =
+val noRepeats : #a:Type0 -> list a -> Tot bool
+let rec noRepeats #a la =
   match la with
   | [] -> true
-  | h :: tl ->  not(mem h tl) && noRepeats tl
-
+  | h :: tl -> not(mem h tl) && noRepeats tl
 
 (** List of tuples **)
-
-val assoc: 'a -> list ('a*'b) -> Tot (option 'b)
-let rec assoc a x = match x with
+val assoc: #a:Type0 -> #b:Type -> a -> list (Tuple2 a b) -> Tot (option b)
+let rec assoc #a #b (x:a) = function
   | [] -> None
-  | (a', b)::tl -> if a=a' then Some b else assoc a tl
+  | (x', y)::tl -> if x=x' then Some y else assoc x tl
 
-val split: list ('a * 'b) -> Tot (list 'a * list 'b)
+val split: list (Tuple2 'a 'b) -> Tot (list 'a * list 'b)
 let rec split l = match l with
     | [] -> ([],[])
     | (hd1,hd2)::tl ->
@@ -196,7 +196,7 @@ let rec split l = match l with
        (hd1::tl1,hd2::tl2)
 let unzip = split
 
-val unzip3: list ('a * 'b * 'c) -> Tot (list 'a * list 'b * list 'c)
+val unzip3: list (Tuple3 'a 'b 'c) -> Tot (list 'a * list 'b * list 'c)
 let rec unzip3 l = match l with
     | [] -> ([],[],[])
     | (hd1,hd2,hd3)::tl ->
@@ -205,9 +205,10 @@ let rec unzip3 l = match l with
 
 (** Sorting (implemented as quicksort) **)
 val partition_length: f:('a -> Tot bool)
-                  -> l:list 'a
-                  -> Lemma (requires True)
-                           (ensures (length (fst (partition f l)) + length (snd (partition f l)) = length l))
+                    -> l:list 'a
+                    -> Lemma (requires True)
+                            (ensures (length (fst (partition f l))
+                                      + length (snd (partition f l)) = length l))
 let rec partition_length f l = match l with
   | [] -> ()
   | hd::tl -> partition_length f tl
