lib/prims.fst
@@ -1,5 +1,5 @@
 (*
-   Copyright 2008-2014 Nikhil Swamy and Microsoft Research
+   Copyright 2008-2016 Nikhil Swamy and Microsoft Research
 
    Licensed under the Apache License, Version 2.0 (the "License");
    you may not use this file except in compliance with the License.
@@ -14,61 +14,95 @@
    limitations under the License.
 *)
 module Prims
+(* False is the empty inductive type *)
+type False =
 
-kind Unop  = Type -> Type
-kind Binop = Type -> Type -> Type
-type bool
-logic type EqTyp : Type -> Type -> Type          (* infix binary '==' *)
-type Eq2 : #a:Type -> #b:Type -> a -> b -> Type    (* infix binary '==' *)
-opaque logic type b2t (b:bool) = (b == true)
-
-//We assume the Tot effect here; its definition appears a few lines below
-(* Primitive logical connectives *)
+(* True is the singleton inductive type *)
 type True =
   | T
-logic type False
-opaque type l_imp (p:Type) (q:Type) = p -> Tot q                (* infix binary '==>' *)
-type l_and  (p:Type) (q:Type) =
-  | And : p -> q -> (p /\ q)                                      (* infix binary '/\' *)
-type l_or   (p:Type) (q:Type) =                                 (* infix binary '\/' *)
-  | Left : p -> (p \/ q)
-  | Right : q -> (p \/ q)
-opaque type l_iff (p:Type) (q:Type) = (p ==> q) /\ (q ==> p)        (* infix binary '<==>' *)
-opaque type l_not (p:Type) = p ==> False                        (* prefix unary '~' *)
-opaque type Forall (#a:Type) (p:a -> Type) = x:a -> Tot (p x)   (* forall (x:a). p x *)
-type DTuple2: a:Type
-          ->  b:(a -> Type)
-          -> Type =
-  | MkDTuple2: #a:Type
-           ->  #b:(a -> Type)
-           -> _1:a
-           -> _2:b _1
-           -> DTuple2 a b
-opaque type Exists (#a:Type) (p:a -> Type) = x:a & p x          (* exists (x:a). p x *)
-logic type XOR (p:Type) (q:Type) = (p \/ q) /\ ~(p /\ q)
-opaque type ITE (p:Type) (q:Type) (r:Type) = (p ==> q) /\ (~p ==> r) (* if/then/else in concrete syntax *)
-logic type ForallTyp : (Type -> Type) -> Type (* Handled specially to support quantification over types of arbitrary kinds *)
-logic type ExistsTyp : (Type -> Type) -> Type (* Handled specially to support quantification over types of arbitrary kinds *)
-logic type Precedes : #a:Type -> #b:Type -> a -> b -> Type  (* a built-in well-founded partial order over all terms *)
+
+(* another singleton type, with its only inhabitant written '()'
+   we assume it is primitive, for convenient interop with other languages *)
+assume new type unit : Type0
+
+(*
+   infix binary '==';
+   proof irrelevant, heterogeneous equality in Type#0;
+   primitive (TODO: make it an inductive?)
+*)
+assume type Eq2 : #a:Type -> #b:Type -> a -> b -> Type0
+
+(* bool is a two element type with elements {'true', 'false'}
+   we assume it is primitive, for convenient interop with other languages *)
+assume new type bool : Type0
+
+(* bool-to-type coercion *)
+opaque type b2t (b:bool) = (b == true)
+
+(* constructive conjunction *)
+type c_and  (p:Type) (q:Type) =
+  | And   : p -> q -> c_and p q
+
+(* '/\'  : specialized to Type#0 *)
+opaque type l_and (p:Type0) (q:Type0) = c_and p q
+
+(* constructive disjunction *)
+type c_or   (p:Type) (q:Type) =
+  | Left  : p -> c_or p q
+  | Right : q -> c_or p q
+
+(* '\/'  : specialized to Type#0 *)
+opaque type l_or (p:Type0) (q:Type0) = c_or p q
+
+(* '==>' : specialized to Type#0 *)
+opaque type l_imp (p:Type0) (q:Type0) = p -> Tot q
+                                         (* ^^^ NB: The Tot effect is primitive;            *)
+				         (*         elaborated using PURE a few lines below *)
+(* infix binary '<==>' *)
+opaque type l_iff (p:Type) (q:Type) = (p ==> q) /\ (q ==> p)
+
+(* prefix unary '~' *)
+opaque type l_not (p:Type) = p ==> False
+
+type XOR (p:Type) (q:Type) = (p \/ q) /\ ~(p /\ q)
+
+opaque type ITE (p:Type) (q:Type) (r:Type) = (p ==> q) /\ (~p ==> r)
+
+(* infix binary '<<'; a built-in well-founded partial order over all terms *)
+assume type precedes : #a:Type -> #b:Type -> a -> b -> Type0
+
+(* A coercion down to universe 0 *)
+type squash (p:Type) = u:unit{p}
+
+(* forall (x:a). p x : specialized to Type#0 *)
+opaque type Forall (#a:Type) (p:a -> Type0) = squash (x:a -> Tot (p x))
+
+(* dependent pairs DTuple2 in concrete syntax is '(x:a & b x)' *)
+type DTuple2 (a:Type)
+             (b:(a -> Type)) =
+  | MkDTuple2: _1:a
+            -> _2:b _1
+            -> DTuple2 a b
+
+(* exists (x:a). p x : specialized to Type#0 *)
+opaque type Exists (#a:Type) (p:a -> Type0) = squash (x:a & p x)
 
 (* PURE effect *)
-kind PurePre = Type
-kind PurePost (a:Type) = a -> Type
-kind PureWP   (a:Type) = PurePost a -> PurePre
+type PurePre = Type0
+type PurePost (a:Type) = a -> Type0
+type PureWP   (a:Type) = PurePost a -> Tot PurePre
 type pure_return (a:Type) (x:a) (p:PurePost a) =
      p x
 type pure_bind_wlp (a:Type) (b:Type)
-                   (wlp1:PureWP a) (wlp2:(a -> PureWP b))
+                   (wlp1:PureWP a) (wlp2:(a -> Tot (PureWP b)))
                    (p:PurePost b) =
      wlp1 (fun (x:a) -> wlp2 x p)
 type pure_bind_wp  (a:Type) (b:Type)
                    (wp1:PureWP a) (wlp1:PureWP a)
-                   (wp2: (a -> PureWP b)) (wlp2: (a -> PureWP b)) =
+                   (wp2: (a -> Tot (PureWP b))) (wlp2: (a -> Tot (PureWP b))) =
      pure_bind_wlp a b wp1 wp2
 type pure_if_then_else (a:Type) (p:Type) (wp_then:PureWP a) (wp_else:PureWP a) (post:PurePost a) =
-     (if p
-      then wp_then post
-      else wp_else post)
+     ITE p (wp_then post) (wp_else post)
 type pure_ite_wlp (a:Type) (wlp_cases:PureWP a) (post:PurePost a) =
      (forall (x:a). wlp_cases (fun (x':a) -> ~(Eq2 #a #a x x')) \/ post x)
 type pure_ite_wp (a:Type) (wlp_cases:PureWP a) (wp_cases:PureWP a) (post:PurePost a) =
@@ -76,13 +110,12 @@ type pure_ite_wp (a:Type) (wlp_cases:PureWP a) (wp_cases:PureWP a) (post:PurePos
     /\ wp_cases (fun (x:a) -> True)
 type pure_wp_binop (a:Type) (wp1:PureWP a) (op:(Type -> Type -> Type)) (wp2:PureWP a) (p:PurePost a) =
      op (wp1 p) (wp2 p)
-type pure_wp_as_type (a:Type) (wp:PureWP a) = (forall (p:PurePost a). wp p)
-type pure_close_wp (a:Type) (b:Type) (wp:(b -> PureWP a)) (p:PurePost a) = (forall (b:b). wp b p)
-type pure_close_wp_t (a:Type) (wp:(Type -> PureWP a)) (p:PurePost a) = (forall (b:Type). wp b p)
-type pure_assert_p (a:Type) (q:Type) (wp:PureWP a) (p:PurePost a) = (q /\ wp p)
-type pure_assume_p (a:Type) (q:Type) (wp:PureWP a) (p:PurePost a) = (q ==> wp p)
-type pure_null_wp (a:Type) (p:PurePost a) = (forall (x:a). p x)
-type pure_trivial (a:Type) (wp:PureWP a) = wp (fun (x:a) -> True)
+type pure_wp_as_type (a:Type) (wp:PureWP a) = forall (p:PurePost a). wp p
+type pure_close_wp (a:Type) (b:Type) (wp:(b -> Tot (PureWP a))) (p:PurePost a) = forall (b:b). wp b p
+type pure_assert_p (a:Type) (q:Type) (wp:PureWP a) (p:PurePost a) = q /\ wp p
+type pure_assume_p (a:Type) (q:Type) (wp:PureWP a) (p:PurePost a) = q ==> wp p
+type pure_null_wp  (a:Type) (p:PurePost a) = forall (x:a). p x
+type pure_trivial  (a:Type) (wp:PureWP a) = wp (fun (x:a) -> True)
 
 total new_effect { (* The definition of the PURE effect is fixed; no user should ever change this *)
   PURE : a:Type -> wp:PureWP a -> wlp:PureWP a -> Effect
@@ -95,16 +128,16 @@ total new_effect { (* The definition of the PURE effect is fixed; no user should
      ; wp_binop     = pure_wp_binop
      ; wp_as_type   = pure_wp_as_type
      ; close_wp     = pure_close_wp
-     ; close_wp_t   = pure_close_wp_t
      ; assert_p     = pure_assert_p
      ; assume_p     = pure_assume_p
      ; null_wp      = pure_null_wp
      ; trivial      = pure_trivial
 }
+
 effect Pure (a:Type) (pre:PurePre) (post:PurePost a) =
         PURE a
-             (fun (p:PurePost a) -> pre /\ (forall (x:a). post x ==> p x)) (* PureWP *)
-             (fun (p:PurePost a) -> forall (x:a). pre /\ post x ==> p x)   (* WLP *)
+             (fun (p:PurePost a) -> pre /\ (forall (x:a). post x ==> p x)) // PureWP
+             (fun (p:PurePost a) -> forall (x:a). pre /\ post x ==> p x)   // WLP
 effect Admit (a:Type) = PURE a (fun (p:PurePost a) -> True) (fun (p:PurePost a) -> True)
 default effect Tot (a:Type) = PURE a (pure_null_wp a) (pure_null_wp a)
 
@@ -117,41 +150,32 @@ effect Ghost (a:Type) (pre:Type) (post:PurePost a) =
            (fun (p:PurePost a) -> pre /\ (forall (x:a). post x ==> p x))
            (fun (p:PurePost a) -> forall (x:a). pre /\ post x ==> p x)
 
-type unit
-type int
-assume logic val op_AmpAmp             : bool -> bool -> Tot bool
-assume logic val op_BarBar             : bool -> bool -> Tot bool
-assume logic val op_Negation           : bool -> Tot bool
-assume logic val op_Multiply           : int -> int -> Tot int
-assume logic val op_Subtraction        : int -> int -> Tot int
-assume logic val op_Addition           : int -> int -> Tot int
-assume logic val op_Minus              : int -> Tot int
-assume logic val op_LessThanOrEqual    : int -> int -> Tot bool
-assume logic val op_GreaterThan        : int -> int -> Tot bool
-assume logic val op_GreaterThanOrEqual : int -> int -> Tot bool
-assume logic val op_LessThan           : int -> int -> Tot bool
+assume new type int : Type0
+assume val op_AmpAmp             : bool -> bool -> Tot bool
+assume val op_BarBar             : bool -> bool -> Tot bool
+assume val op_Negation           : bool -> Tot bool
+assume val op_Multiply           : int -> int -> Tot int
+assume val op_Subtraction        : int -> int -> Tot int
+assume val op_Addition           : int -> int -> Tot int
+assume val op_Minus              : int -> Tot int
+assume val op_LessThanOrEqual    : int -> int -> Tot bool
+assume val op_GreaterThan        : int -> int -> Tot bool
+assume val op_GreaterThanOrEqual : int -> int -> Tot bool
+assume val op_LessThan           : int -> int -> Tot bool
 (* Primitive (structural) equality.
-   What about for function types? *)
-assume val op_Equality :    #a:Type -> a -> a -> Tot bool
-assume val op_disEquality : #a:Type -> a -> a -> Tot bool
-
-type int16 = i:int{i > -32769  /\ 32768 > i}
-type int32 = int
-type int64
-type uint8
-type uint16
-type uint32
-type uint64
-type char
-type float
-type string
-type array : Type -> Type
-assume val strcat : string -> string -> Tot string
-assume logic type LBL : string -> Type -> Type
-type exn
-type HashMultiMap : Type -> Type -> Type //needed for bootstrapping
-type byte = uint8
+   Restricted to small types.
+   But, still allows functions ... TODO: disallow functions *)
+assume val op_Equality :    #a:Type0 -> a -> a -> Tot bool
+assume val op_disEquality : #a:Type0 -> a -> a -> Tot bool
+assume new type char   : Type0
+assume new type float  : Type0
+assume new type string : Type0
+assume new type exn : Type0
 type double = float
+
+assume val strcat : string -> string -> Tot string
+assume new type uint8 : Type0
+type byte = uint8
 
 type list (a:Type) =
   | Nil  : list a
@@ -160,12 +184,9 @@ type list (a:Type) =
 type pattern =
   | SMTPat   : #a:Type -> a -> pattern
   | SMTPatT  : a:Type -> pattern
-  | SMTPatOr : list (list pattern) -> pattern
+//  | SMTPatOr : list (list pattern) -> pattern //TODO: rechecking this fails some universe checks
 
-assume type decreases : #a:Type -> a -> Type
-
-effect Lemma (a:Type) (pre:Type) (post:Type) (pats:list pattern) =
-       Pure a pre (fun r -> post)
+assume type decreases : #a:Type -> a -> Type0
 
 (*
    Lemma is desugared specially. You can write:
@@ -173,6 +194,10 @@ effect Lemma (a:Type) (pre:Type) (post:Type) (pats:list pattern) =
      Lemma phi                 for   Lemma (requires True) phi []
      Lemma t1..tn              for   Lemma unit t1..tn
 *)
+effect Lemma (a:Type) (pre:Type) (post:Type) (pats:list pattern) =
+       Pure a pre (fun r -> post)
+
+
 type option (a:Type) =
   | None : option a
   | Some : v:a -> option a
@@ -196,28 +221,28 @@ default effect Dv (a:Type) =
      DIV a (fun (p:PurePost a) -> (forall (x:a). p x))
            (fun (p:PurePost a) -> (forall (x:a). p x))
 
-kind STPre_h  (heap:Type)          = heap -> Type
-kind STPost_h (heap:Type) (a:Type) = a -> heap-> Type
-kind STWP_h   (heap:Type) (a:Type) = STPost_h heap a -> STPre_h heap
+type STPre_h  (heap:Type)          = heap -> Type0
+type STPost_h (heap:Type) (a:Type) = a -> heap -> Type0
+type STWP_h   (heap:Type) (a:Type) = STPost_h heap a -> Tot (STPre_h heap)
 
 type st_return        (heap:Type) (a:Type)
                       (x:a) (p:STPost_h heap a) =
      p x
 type st_bind_wp       (heap:Type) (a:Type) (b:Type)
                       (wp1:STWP_h heap a) (wlp1:STWP_h heap a)
-                      (wp2:(a -> STWP_h heap b)) (wlp2:(a -> STWP_h heap b))
+                      (wp2:(a -> Tot (STWP_h heap b))) (wlp2:(a -> Tot (STWP_h heap b)))
                       (p:STPost_h heap b) (h0:heap) =
      wp1 (fun a -> wp2 a p) h0
 type st_bind_wlp      (heap:Type) (a:Type) (b:Type)
-                      (wlp1:STWP_h heap a) (wlp2:(a -> STWP_h heap b))
+                      (wlp1:STWP_h heap a) (wlp2:(a -> Tot (STWP_h heap b)))
                       (p:STPost_h heap b) (h0:heap) =
      wlp1 (fun a -> wlp2 a p) h0
 type st_if_then_else  (heap:Type) (a:Type) (p:Type)
                       (wp_then:STWP_h heap a) (wp_else:STWP_h heap a)
                       (post:STPost_h heap a) (h0:heap) =
-     (if p
-      then wp_then post h0
-      else wp_else post h0)
+     ITE p
+        (wp_then post h0)
+	(wp_else post h0)
 type st_ite_wlp       (heap:Type) (a:Type)
                       (wlp_cases:STWP_h heap a)
                       (post:STPost_h heap a) (h0:heap) =
@@ -238,13 +263,9 @@ type st_wp_binop      (heap:Type) (a:Type)
 type st_wp_as_type    (heap:Type) (a:Type) (wp:STWP_h heap a) =
      (forall (p:STPost_h heap a) (h:heap). wp p h)
 type st_close_wp      (heap:Type) (a:Type) (b:Type)
-                      (wp:(b -> STWP_h heap a))
+                      (wp:(b -> Tot (STWP_h heap a)))
                       (p:STPost_h heap a) (h:heap) =
      (forall (b:b). wp b p h)
-type st_close_wp_t    (heap:Type) (a:Type)
-                      (wp:(Type -> STWP_h heap a))
-                      (p:STPost_h heap a) (h:heap) =
-     (forall (b:Type). wp b p h)
 type st_assert_p      (heap:Type) (a:Type) (p:Type)
                       (wp:STWP_h heap a)
                       (q:STPost_h heap a) (h:heap) =
@@ -271,7 +292,6 @@ new_effect {
      ; wp_binop     = st_wp_binop heap
      ; wp_as_type   = st_wp_as_type heap
      ; close_wp     = st_close_wp heap
-     ; close_wp_t   = st_close_wp_t heap
      ; assert_p     = st_assert_p heap
      ; assume_p     = st_assume_p heap
      ; null_wp      = st_null_wp heap
@@ -279,23 +299,25 @@ new_effect {
 }
 
 (* Effect EXCEPTION *)
-kind ExPre  = Type
-kind ExPost (a:Type) = result a -> Type
-kind ExWP   (a:Type) = ExPost a -> ExPre
+type ExPre  = Type0
+type ExPost (a:Type) = result a -> Type0
+type ExWP   (a:Type) = ExPost a -> Tot ExPre
 type ex_return (a:Type) (x:a) (p:ExPost a) = p (V x)
-type ex_bind_wlp (a:Type) (b:Type) (wlp1:ExWP a) (wlp2:(a -> ExWP b)) (p:ExPost b) =
-   (forall (rb:result b). p rb \/ wlp1 (fun ra1 -> if b2t (is_V ra1)
-                                                      then wlp2 (V.v ra1) (fun rb2 -> rb2=!=rb)
-                                                      else  ra1 =!= rb))
-type ex_bind_wp (a:Type) (b:Type) (wp1:ExWP a) (wlp1:ExWP a) (wp2:(a -> ExWP b)) (wlp2:(a -> ExWP b)) (p:ExPost b) =
+type ex_bind_wlp (a:Type) (b:Type) (wlp1:ExWP a) (wlp2:(a -> Tot (ExWP b))) (p:ExPost b) =
+   (forall (rb:result b). p rb \/ wlp1 (fun ra1 -> if is_V ra1
+                                          then wlp2 (V.v ra1) (fun rb2 -> rb2=!=rb)
+                                          else ra1 =!= rb))
+type ex_bind_wp (a:Type) (b:Type)
+		(wp1:ExWP a) (wlp1:ExWP a)
+		(wp2:(a -> Tot (ExWP b))) (wlp2:(a -> Tot (ExWP b))) (p:ExPost b) =
    ex_bind_wlp a b wlp1 wlp2 p
-   /\ wp1 (fun ra1 -> (ITE (b2t (is_V ra1))
-                            (wp2 (V.v ra1) (fun rb2 -> True))
-                             True))
+   /\ wp1 (fun ra1 -> if is_V ra1
+                   then wp2 (V.v ra1) (fun rb2 -> True)
+                   else True)
 type ex_if_then_else (a:Type) (p:Type) (wp_then:ExWP a) (wp_else:ExWP a) (post:ExPost a) =
-   (if p
-    then wp_then post
-    else wp_else post)
+   ITE p
+       (wp_then post)
+       (wp_else post)
 type ex_ite_wlp  (a:Type) (wlp_cases:ExWP a) (post:ExPost a) =
     (forall (a:result a). wlp_cases (fun a1 -> a=!=a1) \/ post a)
 type ex_ite_wp (a:Type) (wlp_cases:ExWP a) (wp_cases:ExWP a) (post:ExPost a) =
@@ -304,8 +326,7 @@ type ex_ite_wp (a:Type) (wlp_cases:ExWP a) (wp_cases:ExWP a) (post:ExPost a) =
 type ex_wp_binop (a:Type) (wp1:ExWP a) (op:(Type -> Type -> Type)) (wp2:ExWP a) (p:ExPost a) =
    op (wp1 p) (wp2 p)
 type ex_wp_as_type (a:Type) (wp:ExWP a) = (forall (p:ExPost a). wp p)
-type ex_close_wp (a:Type) (b:Type) (wp:(b -> ExWP a)) (p:ExPost a) = (forall (b:b). wp b p)
-type ex_close_wp_t (a:Type) (wp:(Type -> ExWP a)) (p:ExPost a)  = (forall (b:Type). wp b p)
+type ex_close_wp (a:Type) (b:Type) (wp:(b -> Tot (ExWP a))) (p:ExPost a) = (forall (b:b). wp b p)
 type ex_assert_p (a:Type) (q:Type) (wp:ExWP a) (p:ExPost a) = (q /\ wp p)
 type ex_assume_p (a:Type) (q:Type) (wp:ExWP a) (p:ExPost a) = (q ==> wp p)
 type ex_null_wp (a:Type) (p:ExPost a) = (forall (r:result a). p r)
@@ -323,7 +344,6 @@ new_effect {
   ; wp_binop     = ex_wp_binop
   ; wp_as_type   = ex_wp_as_type
   ; close_wp     = ex_close_wp
-  ; close_wp_t   = ex_close_wp_t
   ; assert_p     = ex_assert_p
   ; assume_p     = ex_assume_p
   ; null_wp      = ex_null_wp
@@ -331,33 +351,33 @@ new_effect {
 }
 effect Exn (a:Type) (pre:ExPre) (post:ExPost a) =
        EXN a
-         (fun (p:ExPost a) -> pre /\ (forall (r:result a). (pre /\ post r) ==> p r)) (* ExWP *)
-         (fun (p:ExPost a) -> (forall (r:result a). (pre /\ post r) ==> p r))         (* WLP *)
+         (fun (p:ExPost a) -> pre /\ (forall (r:result a). (pre /\ post r) ==> p r)) (* WP *)
+         (fun (p:ExPost a) -> (forall (r:result a). (pre /\ post r) ==> p r))       (* WLP *)
 default effect Ex (a:Type) = Exn a True (fun v -> True)
 
-kind AllPre_h  (h:Type)           = h -> Type
-kind AllPost_h (h:Type) (a:Type)  = result a -> h -> Type
-kind AllWP_h   (h:Type) (a:Type)  = AllPost_h h a -> AllPre_h h
+type AllPre_h  (h:Type)           = h -> Type
+type AllPost_h (h:Type) (a:Type)  = result a -> h -> Type
+type AllWP_h   (h:Type) (a:Type)  = AllPost_h h a -> Tot (AllPre_h h)
 
 type all_return  (heap:Type) (a:Type) (x:a) (p:AllPost_h heap a) = p (V x)
 type all_bind_wp (heap:Type) (a:Type) (b:Type)
                  (wp1:AllWP_h heap a) (wlp1:AllWP_h heap a)
-                 (wp2:(a -> AllWP_h heap b)) (wlp2:(a -> AllWP_h heap b))
+                 (wp2:(a -> Tot (AllWP_h heap b))) (wlp2:(a -> Tot (AllWP_h heap b)))
                  (p:AllPost_h heap b) (h0:heap) =
-   (wp1 (fun ra h1 -> b2t(is_V ra) ==> wp2 (V.v ra) p h1) h0)
+   (wp1 (fun ra h1 -> is_V ra ==> wp2 (V.v ra) p h1) h0)
 type all_bind_wlp (heap:Type) (a:Type) (b:Type)
-                  (wlp1:AllWP_h heap a) (wlp2:(a -> AllWP_h heap b))
+                  (wlp1:AllWP_h heap a) (wlp2:(a -> Tot (AllWP_h heap b)))
                   (p:AllPost_h heap b) (h0:heap) =
    (forall rb h. wlp1 (fun ra h1 ->
-       if b2t (is_V ra)
+       if is_V ra
        then wlp2 (V.v ra) (fun rb2 h2 -> rb=!=rb2 \/ h=!=h2) h1
        else rb=!=ra \/ h=!=h1) h0 \/ p rb h)
 type all_if_then_else (heap:Type) (a:Type) (p:Type)
                       (wp_then:AllWP_h heap a) (wp_else:AllWP_h heap a)
                       (post:AllPost_h heap a) (h0:heap) =
-   (if p
-    then wp_then post h0
-    else wp_else post h0)
+   ITE p
+       (wp_then post h0)
+       (wp_else post h0)
 type all_ite_wlp  (heap:Type) (a:Type)
                   (wlp_cases:AllWP_h heap a)
                   (post:AllPost_h heap a) (h0:heap) =
@@ -374,13 +394,9 @@ type all_wp_binop (heap:Type) (a:Type)
 type all_wp_as_type (heap:Type) (a:Type) (wp:AllWP_h heap a) =
     (forall (p:AllPost_h heap a) (h:heap). wp p h)
 type all_close_wp (heap:Type) (a:Type) (b:Type)
-                  (wp:(b -> AllWP_h heap a))
+                  (wp:(b -> Tot (AllWP_h heap a)))
                   (p:AllPost_h heap a) (h:heap) =
     (forall (b:b). wp b p h)
-type all_close_wp_t (heap:Type) (a:Type)
-                    (wp:(Type -> AllWP_h heap a))
-                    (p:AllPost_h heap a) (h:heap) =
-    (forall (b:Type). wp b p h)
 type all_assert_p (heap:Type) (a:Type) (p:Type)
                   (wp:AllWP_h heap a) (q:AllPost_h heap a) (h:heap) =
     p /\ wp q h
@@ -405,12 +421,10 @@ new_effect {
   ; wp_binop     = all_wp_binop     heap
   ; wp_as_type   = all_wp_as_type   heap
   ; close_wp     = all_close_wp     heap
-  ; close_wp_t   = all_close_wp_t   heap
   ; assert_p     = all_assert_p     heap
   ; assume_p     = all_assume_p     heap
   ; null_wp      = all_null_wp      heap
   ; trivial      = all_trivial      heap
-
 }
 
 sub_effect
@@ -422,17 +436,20 @@ type lex_t =
   | LexTop  : lex_t
   | LexCons : #a:Type -> a -> lex_t -> lex_t
 
+(* 'a * 'b *)
 type Tuple2 'a 'b =
   | MkTuple2: _1:'a
            -> _2:'b
            -> Tuple2 'a 'b
 
+(* 'a * 'b * 'c *)
 type Tuple3 'a 'b 'c =
   | MkTuple3: _1:'a
            -> _2:'b
            -> _3:'c
           -> Tuple3 'a 'b 'c
 
+(* 'a * 'b * 'c * 'd *)
 type Tuple4 'a 'b 'c 'd =
   | MkTuple4: _1:'a
            -> _2:'b
@@ -440,6 +457,7 @@ type Tuple4 'a 'b 'c 'd =
            -> _4:'d
            -> Tuple4 'a 'b 'c 'd
 
+(* 'a * 'b * 'c * 'd * 'e *)
 type Tuple5 'a 'b 'c 'd 'e =
   | MkTuple5: _1:'a
            -> _2:'b
@@ -448,6 +466,7 @@ type Tuple5 'a 'b 'c 'd 'e =
            -> _5:'e
            -> Tuple5 'a 'b 'c 'd 'e
 
+(* 'a * 'b * 'c * 'd * 'e * 'f *)
 type Tuple6 'a 'b 'c 'd 'e 'f =
   | MkTuple6: _1:'a
            -> _2:'b
@@ -458,6 +477,7 @@ type Tuple6 'a 'b 'c 'd 'e 'f =
            -> Tuple6 'a 'b 'c 'd 'e 'f
 
 
+(* 'a * 'b * 'c * 'd * 'e * 'f * 'g *)
 type Tuple7 'a 'b 'c 'd 'e 'f 'g =
   | MkTuple7: _1:'a
            -> _2:'b
@@ -468,7 +488,7 @@ type Tuple7 'a 'b 'c 'd 'e 'f 'g =
            -> _7:'g
            -> Tuple7 'a 'b 'c 'd 'e 'f 'g
 
-
+(* 'a * 'b * 'c * 'd * 'e * 'f * 'g * 'h *)
 type Tuple8 'a 'b 'c 'd 'e 'f 'g 'h =
   | MkTuple8: _1:'a
            -> _2:'b
@@ -480,49 +500,40 @@ type Tuple8 'a 'b 'c 'd 'e 'f 'g 'h =
            -> _8:'h
            -> Tuple8 'a 'b 'c 'd 'e 'f 'g 'h
 
-type DTuple3: a:Type
-            -> b:(a -> Type)
-            -> c:(x:a -> b x -> Type)
-            -> Type =
-   | MkDTuple3: #a:Type
-            ->  #b:(a -> Type)
-            ->  #c:(x:a -> b x -> Type)
-            -> _1:a
-            -> _2:b _1
-            -> _3:c _1 _2
-            -> DTuple3 a b c
+(* Concrete syntax (x:a & y:b x & c x y) *)
+type DTuple3 (a:Type)
+             (b:(a -> Type))
+             (c:(x:a -> b x -> Type)) =
+   | MkDTuple3:_1:a
+             -> _2:b _1
+             -> _3:c _1 _2
+             -> DTuple3 a b c
 
-type DTuple4: a:Type
-           -> b:(x:a -> Type)
-           -> c:(x:a -> b x -> Type)
-           -> d:(x:a -> y:b x -> z:c x y -> Type)
-           -> Type =
- | MkDTuple4: #a:Type
-           -> #b:(a -> Type)
-           -> #c:(x:a -> b x -> Type)
-           -> #d:(x:a -> y:b x -> z:c x y -> Type)
-           -> _1:a
+(* Concrete syntax (x:a & y:b x & z:c x y & d x y z) *)
+type DTuple4 (a:Type)
+             (b:(x:a -> Type))
+             (c:(x:a -> b x -> Type))
+             (d:(x:a -> y:b x -> z:c x y -> Type)) =
+ | MkDTuple4:_1:a
            -> _2:b _1
            -> _3:c _1 _2
            -> _4:d _1 _2 _3
            -> DTuple4 a b c d
 
-
 type as_requires (#a:Type) (wp:PureWP a)  = wp (fun x -> True)
-type as_ensures  (#a:Type) (wlp:PureWP a) (x:a) = ~ (wlp (fun y -> ~(y=x)))
+type as_ensures  (#a:Type) (wlp:PureWP a) (x:a) = ~ (wlp (fun y -> (y=!=x)))
 
 val fst : ('a * 'b) -> Tot 'a
 let fst x = MkTuple2._1 x
 
-
 val snd : ('a * 'b) -> Tot 'b
 let snd x = MkTuple2._2 x
 
-val dfst : #a:Type -> #b:(a -> Type) -> DTuple2 a b -> Tot a
-let dfst t = MkDTuple2._1 t
+val dfst : #a:Type -> #b:(a -> Type) -> (x:a & b x) -> Tot a
+let dfst #a #b t = MkDTuple2._1 t
 
-val dsnd : #a:Type -> #b:(a -> Type) -> t:(DTuple2 a b) -> Tot (b (MkDTuple2._1 t))
-let dsnd t = MkDTuple2._2 t
+val dsnd : #a:Type -> #b:(a -> Type) -> t:(x:a & b x) -> Tot (b (MkDTuple2._1 t))
+let dsnd #a #b t = MkDTuple2._2 t
 
 type Let (#a:Type) (x:a) (body:(a -> Type)) = body x
 logic type InductionHyp : #a:Type -> a -> Type -> Type
@@ -538,23 +549,24 @@ assume val cut     : p:Type -> Pure unit (requires $"assertion failed" p) (fun x
 assume val qintro  : #a:Type -> #p:(a -> Type) -> =f:(x:a -> Lemma (p x)) -> Lemma (forall (x:a). p x)
 assume val ghost_lemma: #a:Type -> #p:(a -> Type) -> #q:(a -> unit -> Type) -> =f:(x:a -> Ghost unit (p x) (q x)) -> Lemma (forall (x:a). p x ==> q x ())
 assume val raise: exn -> Ex 'a       (* TODO: refine with the Exn monad *)
-val ignore: 'a -> Tot unit
-let ignore x = ()
+val ignore: #a:Type -> a -> Tot unit
+let ignore #a x = ()
 
 type nat = i:int{i >= 0}
 type pos = i:int{i > 0}
 type nonzero = i:int{i<>0}
 
-(* For the moment we require not just that the divisor is non-zero,
-   but also that the dividend is natural. This works around a
-   mismatch between the semantics of integer division in SMT-LIB and
-   in F#/OCaml. For SMT-LIB ints the modulus is always positive (as in
-   math Euclidian division), while for F#/OCaml ints the modulus has
-   the same sign as the dividend. Our arbitrary precision ints don't
-   quite correspond to finite precision F#/OCaml ints though, but to
-   OCaml's big_ints (for which the modulus is always positive).  So
-   we'll need to return to this point anyway, when we discuss how to
-   soundly map F* ints to something in F#/OCaml. *)
+(*    For the moment we require not just that the divisor is non-zero, *)
+(*    but also that the dividend is natural. This works around a *)
+(*    mismatch between the semantics of integer division in SMT-LIB and *)
+(*    in F#/OCaml. For SMT-LIB ints the modulus is always positive (as in *)
+(*    math Euclidian division), while for F#/OCaml ints the modulus has *)
+(*    the same sign as the dividend. Our arbitrary precision ints don't *)
+(*    quite correspond to finite precision F#/OCaml ints though, but to *)
+(*    OCaml's big_ints (for which the modulus is always positive).  So *)
+(*    we'll need to return to this point anyway, when we discuss how to *)
+(*    soundly map F* ints to something in F#/OCaml.  *)
+
 assume val op_Modulus            : int -> nonzero -> Tot int
 assume val op_Division           : nat -> nonzero -> Tot int
 
